# q01c

## 3.
Find the Fourier series representation of $$x(t)=\sum_{k=-\infty}^{\infty}{\sqcap\left(\frac{t-10k}{5}\right)}$$

#### 3.
 - First, find the fundamental frequency.
    - $$f=\frac{1}{T}=\frac{1}{(10)}\:\text{Hz};$$
    - $$T=10\:\text{sec};$$
 - Using this frequency, find the **Fourier Series Coefficients**
$$
    \begin{align*}
    X_n&=\frac{1}{T}\int_{-\infty}^{\infty}{\left(\sqcap{\left(\frac{t}{5}\right)e^{-j\frac{2\pi{n}t}{T}}}\right)dt}&&\left<T=10\right>\\
    &=\frac{1}{(10)}\int_{-5}^{5}{\left(\sqcap{\left(\frac{t}{5}\right)e^{-j\frac{2\pi{n}t}{(10)}}}\right)dt}\\
    &=\left.\frac{1}{10}(5)\text{sinc}{\left(5f\right)}\right|_{f=\frac{n}{T}=\frac{n}{10}}=\frac{5}{10}\text{sinc}{\left(\frac{5n}{10}\right)}\\
    &=\frac{1}{2}\text{sinc}{\left(\frac{n}{2}\right)}\\
    x(t)&=\sum_{n=-\infty}^{\infty}{X_n}e^{-j\frac{2\pi{n}t}{T}}=\sum_{n=-\infty}^{\infty}{\left(\frac{1}{2}\text{sinc}{\left(\frac{n}{2}\right)}\right)}e^{-j\frac{2\pi{n}t}{10}}
    \end{align*}
$$
Note that
$$
    \left\{
    \begin{align*}
    X_n&=\frac{1}{2}\text{sinc}{\left(\frac{n}{2}\right)}=\frac{1}{2}\frac{\sin{(\pi\left(\frac{n}{2}\right))}}{(\pi\left(\frac{n}{2}\right))}=\frac{\sin{(\pi\left(\frac{n}{2}\right))}}{(n\pi)}\\
    X_{0}&=\frac{1}{2};\\
    X_{2n}&=0;\\
    X_{2n+1}&=\frac{\sin{(\pi\left(\frac{(2n+1)}{2}\right))}}{((2n+1)\pi)}=\frac{(-1)^k}{\pi(2n+1)};&&\text{for }|n|=0,1,\cdots\\\vdots\\
    &\left<\:\:\:\:\begin{matrix}n=1:&\sin{(1.5\pi)}=-1\\n=2:&\sin{(2.5\pi)}=1\\\vdots&\vdots\end{matrix}\:\:\:\:\right>\\\vdots\\
    \end{align*}
    \right\}
$$
Therefore we can modify our original equation into such.
$$
    \begin{align*}
    x(t)&=\sum_{n=-\infty}^{\infty}{\left(\frac{1}{2}\text{sinc}{\left(\frac{n}{2}\right)}\right)}e^{-j\frac{2\pi{n}t}{10}}\\
    &=X_0+\left(\sum_{-\infty}^{0}{\frac{(-1)^k}{\pi(2n+1)}}e^{-j\frac{2\pi{(2n+1)}t}{10}}+\sum_{0}^{\infty}{\frac{(-1)^k}{\pi(2n+1)}}e^{-j\frac{2\pi{(2n+1)}t}{10}}\right)\\
    &\left<\:\:\:\:\begin{matrix}n=-1:&\sin{(-1.5\pi)}=1\\n=-2:&\sin{(-2.5\pi)}=-1\\\vdots&\vdots\end{matrix}\:\:\:\:\right>\\
    &=\left(\frac{1}{2}\right)+\sum_{n=0}^{\infty}{\left(\frac{(-1)^k}{\pi(2n+1)}\right)}\left[e^{j\frac{2\pi{(2n+1)}t}{10}}+e^{-j\frac{2\pi{(2n+1)}t}{10}}\right]\\\vdots\\
    &\left<\cos{(a)}=\frac{1}{2}\left[e^{-ja}+e^{ja}\right]\right>\\\vdots\\
    &=\left(\frac{1}{2}\right)+2\sum_{n=0}^{\infty}{\left(\frac{(-1)^k}{\pi(2n+1)}\right)}\cos{\left(\frac{2\pi(2n+1)}{10}\right)}

    \end{align*}
$$